some progress

Cslib/Computability/Automata/EpsilonNA/ToNA.lean
@@ -41,20 +41,84 @@ variable {State Symbol : Type*}
 def toNAFinAcc (a : εNA.FinAcc State Symbol) : NA.FinAcc State Symbol where
   start := a.εClosure a.start
   accept := a.accept
-  Tr := a.saturate.noε.Tr
+  Tr s μ s' := a.STr s (some μ) s'
 
 open Acceptor in
-open scoped NA.FinAcc in
+open scoped NA.FinAcc LTS LTS.STr LTS.SMTr in
 /-- Correctness of `toNAFinAcc`. -/
 @[scoped grind _=_]
 theorem toNAFinAcc_language_eq {ena : εNA.FinAcc State Symbol} :
     language ena.toNAFinAcc = language ena := by
   ext xs
-  have : ∀ s s', ena.saturate.MTr s (xs.map some) s' = ena.saturate.noε.MTr s xs s' := by
-    simp [LTS.noε_saturate_mTr]
-  #adaptation_note
-  /-- A grind regression found moving to nightly-2026-03-31 (changes from lean#13166) -/
-  grind [Accepts]
+  cases xs
+  case nil =>
+    apply Iff.intro <;> intro h
+    case mp =>
+      rcases h with ⟨s, hs, s', hs', h⟩
+      simp only [toNAFinAcc, εClosure, LTS.τClosure, LTS.setImage, LTS.saturate, Set.mem_iUnion,
+        exists_prop] at hs
+      rcases hs with ⟨sStart, hStart, hs⟩
+      exists sStart
+      apply And.intro
+      case left => grind
+      case right =>
+        exists s'
+        apply And.intro
+        case left => grind
+        case right =>
+          simp only [List.pure_def, List.bind_eq_flatMap, List.flatMap_nil]
+          grind [LTS.SMTr.τ]
+    case mpr =>
+      rcases h with ⟨s, hs, s', hs', h⟩
+      simp only [List.pure_def, List.bind_eq_flatMap, List.flatMap_nil] at h
+      simp [Accepts]
+      exists s'
+      constructor
+      · simp [toNAFinAcc, εClosure, LTS.τClosure, LTS.saturate]
+        simp [LTS.setImage]
+        exists s
+        constructor
+        · grind
+        · simp [LTS.image]
+          cases h
+          grind
+      · exists s'
+        constructor
+        · grind
+        · grind
+  case cons x xs =>
+    have : ∀ {s s'}, ena.toNAFinAcc.MTr s (x :: xs) s' = ena.SMTr s (x :: xs) s' := by
+      intro s s'
+      have := LTS.sMTr_mTr_not_nil (lts := ena.toLTS) (s := s) (s' := s') (μs := some x :: xs.map some) (by simp)
+      ext
+      apply Iff.intro <;> intro h
+      · simp
+
+      · sorry
+    simp [Accepts]
+    apply Iff.intro <;> intro h
+    · rcases h with ⟨s, hs, s', hs', h⟩
+      rw [this] at h
+      simp [toNAFinAcc] at hs
+      have h_start : ∃ sStart ∈ ena.start, ena.τSTr s sStart := by
+        sorry
+      rcases h_start with ⟨sStart, h_sStart, h_start⟩
+      exists sStart
+      apply And.intro
+      · grind
+      · exists s'
+        apply And.intro
+        · grind
+        · grind
+    -- simp [LTS.noε_saturate_mTr]
+    -- #adaptation_note
+    -- /-- A grind regression found moving to nightly-2026-03-31 (changes from lean#13166) -/
+    -- grind [Accepts]
+  -- have : ∀ s s', ena.MTr s (xs.map some) s' = ena.εMTr s xs s' := by
+  --   simp [LTS.noε_saturate_mTr]
+  -- #adaptation_note
+  -- /-- A grind regression found moving to nightly-2026-03-31 (changes from lean#13166) -/
+  -- grind [Accepts]
 
 end Automata.εNA.FinAcc
 
