Cslib/Foundations/Semantics/LTS/HasTau.lean
@@ -31,8 +31,8 @@ def τSTr [HasTau Label] (lts : LTS State Label) : State → State → Prop :=
 
 /-- Saturated transition relation. -/
 inductive STr [HasTau Label] (lts : LTS State Label) : State → Label → State → Prop where
-| refl : lts.STr s HasTau.τ s
-| tr : lts.τSTr s1 s2 → lts.Tr s2 μ s3 → lts.τSTr s3 s4 → lts.STr s1 μ s4
+  | refl : lts.STr s HasTau.τ s
+  | tr : lts.τSTr s1 s2 → lts.Tr s2 μ s3 → lts.τSTr s3 s4 → lts.STr s1 μ s4
 
 /-- The `LTS` obtained by saturating the transition relation in `lts`. -/
 @[scoped grind =]
@@ -44,14 +44,14 @@ theorem saturate_tr_sTr [HasTau Label] {lts : LTS State Label} :
   lts.saturate.Tr = lts.STr := by rfl
 
 /-- Any transition is also a saturated transition. -/
-theorem STr.single [HasTau Label] (lts : LTS State Label) :
+theorem STr.single [HasTau Label] {lts : LTS State Label} :
     lts.Tr s μ s' → lts.STr s μ s' := by
   intro h
   apply STr.tr .refl h .refl
 
 /-- STr transitions labeled by HasTau.τ are exactly the τSTr transitions. -/
 theorem sTr_τSTr [HasTau Label] (lts : LTS State Label) :
-  lts.STr s HasTau.τ s' ↔ lts.τSTr s s' := by
+    lts.STr s HasTau.τ s' ↔ lts.τSTr s s' := by
   apply Iff.intro <;> intro h
   case mp =>
     cases h
@@ -64,8 +64,8 @@ theorem sTr_τSTr [HasTau Label] (lts : LTS State Label) :
     case tail _ h1 h2 => exact STr.tr h1 h2 .refl
 
 /-- In a saturated LTS, the transition and saturated transition relations are the same. -/
-theorem saturate_τSTr_τSTr [hHasTau : HasTau Label] (lts : LTS State Label)
-  : lts.saturate.τSTr s = lts.τSTr s := by
+theorem saturate_τSTr_τSTr [hHasTau : HasTau Label] (lts : LTS State Label) :
+    lts.saturate.τSTr s = lts.τSTr s := by
   ext s''
   apply Iff.intro <;> intro h
   case mp =>
@@ -82,19 +82,19 @@ theorem saturate_τSTr_τSTr [hHasTau : HasTau Label] (lts : LTS State Label)
 /-- Saturated transitions labelled by τ can be composed. -/
 @[scoped grind .]
 theorem STr.trans_τ
-  [HasTau Label] (lts : LTS State Label)
-  (h1 : lts.STr s1 HasTau.τ s2) (h2 : lts.STr s2 HasTau.τ s3) :
-  lts.STr s1 HasTau.τ s3 := by
+    [HasTau Label] {lts : LTS State Label}
+    (h1 : lts.STr s1 HasTau.τ s2) (h2 : lts.STr s2 HasTau.τ s3) :
+    lts.STr s1 HasTau.τ s3 := by
   rw [sTr_τSTr _] at h1 h2
   rw [sTr_τSTr _]
   apply Relation.ReflTransGen.trans h1 h2
 
 /-- Saturated transitions can be composed. -/
 theorem STr.comp
-  [HasTau Label] (lts : LTS State Label)
-  (h1 : lts.STr s1 HasTau.τ s2)
-  (h2 : lts.STr s2 μ s3)
-  (h3 : lts.STr s3 HasTau.τ s4) :
+    [HasTau Label] {lts : LTS State Label}
+    (h1 : lts.STr s1 HasTau.τ s2)
+    (h2 : lts.STr s2 μ s3)
+    (h3 : lts.STr s3 HasTau.τ s4) :
   lts.STr s1 μ s4 := by
   rw [sTr_τSTr _] at h1 h3
   cases h2
@@ -121,7 +121,7 @@ theorem saturate_tr_saturate_sTr [hHasTau : HasTau Label] (lts : LTS State Label
     case tr hstr1 htr hstr2 =>
       rw [saturate_τSTr_τSTr lts] at hstr1 hstr2
       rw [←sTr_τSTr lts] at hstr1 hstr2
-      exact STr.comp lts hstr1 htr hstr2
+      exact STr.comp hstr1 htr hstr2
 
 /-- In a saturated LTS, every state is in its τ-image. -/
 @[scoped grind .]
@@ -144,6 +144,11 @@ lemma subset_saturate_setImage_τ [HasTau Label] (lts : LTS State Label) :
   intro s h
   grind
 
+/-- `setImage` preserves (non-)emptyness. -/
+@[scoped grind =]
+lemma empty_saturate_setImage_τ [HasTau Label] (lts : LTS State Label) :
+    lts.saturate.setImage S HasTau.τ = ∅ ↔ S = ∅:= by grind
+
 /-- The `τ`-closure of a set of states `S` is the set of states reachable by any state in `S`
 by performing only `τ`-transitions. -/
 def τClosure [HasTau Label] (lts : LTS State Label) (S : Set State) : Set State :=
@@ -158,6 +163,63 @@ lemma τClosure_mem [HasTau Label] (lts : LTS State Label) (h : s ∈ S) :
 @[scoped grind .]
 lemma τClosure_subset [HasTau Label] (lts : LTS State Label) :
     S ⊆ lts.τClosure S := by grind
+
+/-- Saturated multistep transition relation. -/
+inductive SMTr [HasTau Label] (lts : LTS State Label) : State → List Label → State → Prop where
+  | τ : lts.STr s HasTau.τ s' → lts.SMTr s [] s'
+  | stepL : lts.STr s1 μ s2 → lts.SMTr s2 μs s3 → lts.SMTr s1 (μ :: μs) s3
+
+/-- The saturated multistep transition relation is reflexive. -/
+@[scoped grind .]
+theorem SMTr.refl [HasTau Label] (lts : LTS State Label) (s : State) :
+    lts.SMTr s [] s := by grind [LTS.STr, LTS.SMTr]
+
+open scoped LTS.STr
+
+/-- The saturated multistep transition relation is transitive. -/
+@[scoped grind .]
+theorem SMTr.comp [HasTau Label] {lts : LTS State Label}
+    (h₁ : lts.SMTr s₁ μs₁ s₂) (h₂ : lts.SMTr s₂ μs₂ s₃) : lts.SMTr s₁ (μs₁ ++ μs₂) s₃ := by
+  induction h₁
+  case τ s₁ s₂ htr =>
+    cases h₂
+    case τ htr' => grind [SMTr]
+    case stepL _ _ _ μ s₂' μs hstr hmstr =>
+      have hstr' : lts.STr s₁ μ s₂' := by
+        apply STr.comp htr hstr STr.refl
+      simp only [List.nil_append]
+      apply stepL hstr' hmstr
+  case stepL s₁ μ s₁' μs s₂ hstr hmstr ih =>
+    apply stepL hstr (ih h₂)
+
+/-- A multistep transition implies a saturated multistep transition. -/
+@[scoped grind .]
+theorem mTr_sMTr [HasTau Label] {lts : LTS State Label}
+    (h : lts.MTr s μs s') : lts.SMTr s μs s' := by
+  induction μs generalizing s s'
+  case nil => grind [LTS.STr, LTS.SMTr]
+  case cons x xs ih =>
+    cases h
+    case stepL sb htr hmtr => exact SMTr.stepL (STr.single htr) (ih hmtr)
+
+/-- A saturated multistep transition with a nonempty label list implies a multistep transition. -/
+@[scoped grind .]
+theorem sMTr_mTr_not_nil [HasTau Label] {lts : LTS State Label}
+    (hμs : μs ≠ []) (h : lts.SMTr s μs s') : lts.saturate.MTr s μs s' := by
+  induction μs generalizing s
+  case nil => contradiction
+  case cons x xs ih =>
+    cases h
+    case stepL sb htr hmtr =>
+      cases xs with
+      | nil =>
+        cases hmtr
+        case τ h_τ =>
+          exact LTS.MTr.stepL
+            (LTS.STr.comp LTS.STr.refl htr h_τ)
+            LTS.MTr.refl
+      | cons y ys =>
+        exact LTS.MTr.stepL htr (ih (by simp) hmtr)
 
 end LTS
 
