Cslib/Computability/Automata/EpsilonNA/Basic.lean
@@ -46,9 +46,8 @@ namespace FinAcc
 that trace from the start state. -/
 @[scoped grind =]
 instance : Acceptor (FinAcc State Symbol) Symbol where
-  Accepts (a : FinAcc State Symbol) (xs : List Symbol) :=
-    ∃ s ∈ a.εClosure a.start, ∃ s' ∈ a.accept,
-    a.saturate.MTr s (xs.map (some ·)) s'
+    Accepts (a : FinAcc State Symbol) (xs : List Symbol) :=
+  ∃ s ∈ a.start, ∃ s' ∈ a.accept, a.SMTr s xs s'
 
 end FinAcc
 
